_drafts/extract.lean
@@ -1,0 +1,67 @@
+
+/-
+
+How can I extract a fraction of lean into C / rust / verilog.
+I suppose one could deep embed a dsl but that's a lot of work.
+
+
+
+Call yosys.
+ebmc
+
+etc
+
+
+What about verilog -> yosys -> knuckledragger -> lean pipeline?
+
+A little silly, but actually processing the yosys stuff would be pain
+A new lean backend would be the most direct route.
+
+There are worse fates for knuckeldragger than to be a translation hub for lean
+
+-/
+
+import Qq
+import Lean
+open Lean Elab Meta Qq BitVec
+
+-- recursively translate Expr → Verilog ― extend as you need
+partial def exprToVerilog (e : Expr) : MetaM String := do
+  match e with
+  | .lit (.natVal x)      => pure s!"{x}"
+  | _ => throwError "exprToVerilog: unsupported {e}"
+  /-
+  | .app (.app (.const ``BitVec.add ..) a) b =>
+      return s!"({← exprToVerilog a} + {← exprToVerilog b})"
+  | .app (.app (.const ``BitVec.mul ..) a) b =>
+      return s!"({← exprToVerilog a} * {← exprToVerilog b})"
+  | .app (.app (.const ``HAnd ..) a) b =>   -- etc.
+      return s!"({← exprToVerilog a} & {← exprToVerilog b})"
+  | _ => throwError "exprToVerilog: unsupported {e}"
+-/
+
+#check 1#10
+#eval q( 1#10 )
+#check `BitVec.ofNat
+#eval Expr.isAppOf q(1#10) `BitVec.ofNat -- whnf and reduce make junk
+
+def mypat := fun x => BitVec.ofNat x
+def pmatch (pat : Expr) t := do
+  let (vs, _, e1) <- lambdaMetaTelescope pat
+  if <- isDefEq e1 t then
+    vs.mapM instantiateMVars
+  else
+    throwError "pmatch: pattern match failed {pat} {t}"
+
+#eval pmatch q(fun x => BitVec.ofNat x) q(BitVec.ofNat 1)
+
+#eval do
+  let e <- reduce q(1#10)
+  pmatch q(fun x => BitVec.ofNat x) e
+
+--lambdaMetaTelescope mypat
+
+#eval reduce q(1)
+#eval do
+  let e <- reduce q(1)
+  exprToVerilog e
